dependence-schedule/functional-induction-proof.v
@@ -1,4 +1,5 @@
 
+
 (* Me proving statements about maps to understand how to use maps in Coq *)
 
 Require Import FunInd.
@@ -9,8 +10,8 @@ Require Import FunInd FMapInterface.
 
 
 Require Import
-  Coq.FSets.FMapList
-  Coq.Structures.OrderedTypeEx.
+        Coq.FSets.FMapList
+        Coq.Structures.OrderedTypeEx.
 
 Module Import MNat := FMapList.Make(Nat_as_OT).
 Module Import MNatFacts := WFacts(MNat).
@@ -33,42 +34,17 @@ Function insertNats (n: nat)  (mm: NatToNat)  {struct n}: NatToNat :=
   | S (next) => insertNats  next (MNat.add n n mm)
   end.
 
-Theorem insertNatsDoesNotDelete: forall (n: nat) (k: nat) (mm: NatToNat), MNat.In k mm -> MNat.In k (insertNats n mm).
-  intros n. induction n.
+Theorem insertNatsDoesNotDeleteKeys:
+  forall (n: nat) (k: nat) (mm: NatToNat),
+    MNat.In k mm -> MNat.In k (insertNats n mm).
+  intros n.
   intros k mm.
   intros kinmm.
-  simpl.
+  functional induction insertNats n mm.
   exact kinmm.
-  intros k mm.
-  intros k_in_mm.
-
-
-
-Example keys_nonnegative: forall (n: nat) (mm: NatToNat), 
-    forall (k: nat),
-      (MNat.In k mm -> k >= 0) -> 
-      (MNat.In k (insertNats n mm)) -> k >= 0.
-Proof.
-  intros n.
-  induction n.
-  intros mm k kinmm.
-  intros in_oldk.
-  simpl in in_oldk.
-  apply kinmm in in_oldk.
-  intuition.
-  intros mm k kinmm.
-  intros in_insertnats_mm.
-  rewrite elements_in_iff in in_insertnats_mm.
-  destruct in_insertnats_mm.
-  rewrite <- elements_mapsto_iff in H.
-  simpl in H.
-
-  assert (k = S n /\ MNat.In k mm).
-  rewrite -> add_mapsto_iff in H.
-
-  (* Now what?? *)
-
-  (* Either k = (Sn) or K \in mm. If k = Sn then k > 0.
-     if k \in mm, then use kinmm. But, how do I split these two cases? *)
-
-  Admitted.
+  rewrite add_in_iff in IHn0.
+  assert(S next = k \/ MNat.In k mm).
+  auto.
+  apply IHn0.
+  exact H.
+Qed.
